ulib/experimental/Steel.SelEffect.fst
@@ -171,27 +171,29 @@ let bind_req_unnormal (#a:Type)
   (#pre_f:pre_t) (#post_f:post_t a)
   (req_f:req_t pre_f) (ens_f:ens_t pre_f a post_f)
   (#pre_g:a -> pre_t)
+  (#pr:a -> prop)
   (req_g:(x:a -> req_t (pre_g x)))
-  (_:squash (can_be_split_forall post_f pre_g))
+  (_:squash (can_be_split_forall_dep pr post_f pre_g))
   (m0:rmem pre_f)
 = req_f m0 /\
-  (forall (x:a) (m1:rmem (post_f x)). ens_f m0 x m1 ==> (req_g x) (focus_rmem m1 (pre_g x)))
+  (forall (x:a) (m1:rmem (post_f x)). ens_f m0 x m1 ==> pr x /\ (req_g x) (focus_rmem m1 (pre_g x)))
 
 unfold
 let bind_ens_unnormal (#a:Type) (#b:Type)
   (#pre_f:pre_t) (#post_f:post_t a)
   (req_f:req_t pre_f) (ens_f:ens_t pre_f a post_f)
   (#pre_g:a -> pre_t) (#post_g:a -> post_t b)
+  (#pr:a -> prop)
   (ens_g:(x:a -> ens_t (pre_g x) b (post_g x)))
   (post:post_t b)
-  (_:squash (can_be_split_forall post_f pre_g))
+  (_:squash (can_be_split_forall_dep pr post_f pre_g))
   (_:squash (can_be_split_post post_g post))
   (m0:rmem pre_f)
   (y:b)
   (m2:rmem (post y))
 : prop
 = req_f m0 /\
-  (exists (x:a) (m1:rmem (post_f x)). ens_f m0 x m1 /\ (ens_g x) (focus_rmem m1 (pre_g x)) y (focus_rmem m2 (post_g x y)))
+  (exists (x:a) (m1:rmem (post_f x)). pr x /\ ens_f m0 x m1 /\ (ens_g x) (focus_rmem m1 (pre_g x)) y (focus_rmem m2 (post_g x y)))
 
 val bind_aux (a:Type) (b:Type)
   (#pre_f:pre_t) (#post_f:post_t a)
@@ -199,7 +201,8 @@ val bind_aux (a:Type) (b:Type)
   (#pre_g:a -> pre_t) (#post_g:a -> post_t b)
   (#req_g:(x:a -> req_t (pre_g x))) (#ens_g:(x:a -> ens_t (pre_g x) b (post_g x)))
   (#post:post_t b)
-  (#p1:squash (can_be_split_forall post_f pre_g))
+  (#pr:a -> prop)
+  (#p1:squash (can_be_split_forall_dep pr post_f pre_g))
   (#p2:squash (can_be_split_post post_g post))
   (f:repr a pre_f post_f req_f ens_f)
   (g:(x:a -> repr b (pre_g x) (post_g x) (req_g x) (ens_g x)))
@@ -230,7 +233,7 @@ fun frame ->
   y
 
 
-let bind a b #pre_f #post_f #req_f #ens_f #pre_g #post_g #req_g #ens_g #post #p1 #p2 f g =
+let bind a b #pre_f #post_f #req_f #ens_f #pre_g #post_g #req_g #ens_g #post #pr #p1 #p2 f g =
   norm_repr (bind_aux a b f g)
 
 unfold
@@ -326,16 +329,19 @@ let bind_steel_steel_req_unnormal (#a:Type)
   (#pre_f:pre_t) (#post_f:post_t a)
   (req_f:req_t pre_f) (ens_f:ens_t pre_f a post_f)
   (#pre_g:a -> pre_t)
+  (#pr:a -> prop)
   (req_g:(x:a -> req_t (pre_g x)))
   (frame_f:vprop) (frame_g:a -> vprop)
-  (_:squash (can_be_split_forall (fun x -> post_f x `star` frame_f) (fun x -> pre_g x `star` frame_g x)))
+  (_:squash (can_be_split_forall_dep pr
+    (fun x -> post_f x `star` frame_f) (fun x -> pre_g x `star` frame_g x)))
   (m0:rmem (pre_f `star` frame_f))
 = req_f (focus_rmem m0 pre_f) /\
-  (forall (x:a) (m1:rmem (post_f x `star` frame_f)). (
-    can_be_split_trans (post_f x `star` frame_f) (pre_g x `star` frame_g x) (pre_g x);
+  (forall (x:a) (m1:rmem (post_f x `star` frame_f)).
     (ens_f (focus_rmem m0 pre_f) x (focus_rmem m1 (post_f x)) /\
       frame_equalities frame_f (focus_rmem m0 frame_f) (focus_rmem m1 frame_f))
     ==>
+      pr x /\
+      (can_be_split_trans (post_f x `star` frame_f) (pre_g x `star` frame_g x) (pre_g x);
       (req_g x) (focus_rmem m1 (pre_g x))))
 
 unfold
@@ -343,16 +349,19 @@ let bind_steel_steel_ens_unnormal (#a:Type) (#b:Type)
   (#pre_f:pre_t) (#post_f:post_t a)
   (req_f:req_t pre_f) (ens_f:ens_t pre_f a post_f)
   (#pre_g:a -> pre_t) (#post_g:a -> post_t b)
+  (#pr:a -> prop)
   (ens_g:(x:a -> ens_t (pre_g x) b (post_g x)))
   (frame_f:vprop) (frame_g:a -> vprop)
   (post:post_t b)
-  (_:squash (can_be_split_forall (fun x -> post_f x `star` frame_f) (fun x -> pre_g x `star` frame_g x)))
+  (_:squash (can_be_split_forall_dep pr
+    (fun x -> post_f x `star` frame_f) (fun x -> pre_g x `star` frame_g x)))
   (_:squash (can_be_split_post (fun x y -> post_g x y `star` frame_g x) post))
   (m0:rmem (pre_f `star` frame_f))
   (y:b)
   (m2:rmem (post y))
 = req_f (focus_rmem m0 pre_f) /\
-  (exists (x:a) (m1:rmem (post_f x `star` frame_f)). (
+  (exists (x:a) (m1:rmem (post_f x `star` frame_f)).
+    pr x /\ (
     can_be_split_trans (post_f x `star` frame_f) (pre_g x `star` frame_g x) (pre_g x);
     can_be_split_trans (post_f x `star` frame_f) (pre_g x `star` frame_g x) (frame_g x);
     can_be_split_trans (post y) (post_g x y `star` frame_g x) (post_g x y);
@@ -369,7 +378,8 @@ val bind_steel_steel_aux (a:Type) (b:Type)
   (#req_g:(x:a -> req_t (pre_g x))) (#ens_g:(x:a -> ens_t (pre_g x) b (post_g x)))
   (#frame_f:vprop) (#frame_g:a -> vprop)
   (#post:post_t b)
-  (#p:squash (can_be_split_forall
+  (#pr:a -> prop)
+  (#p:squash (can_be_split_forall_dep pr
     (fun x -> post_f x `star` frame_f) (fun x -> pre_g x `star` frame_g x)))
   (#p2:squash (can_be_split_post (fun x y -> post_g x y `star` frame_g x) post))
   (f:repr a pre_f post_f req_f ens_f)
@@ -468,30 +478,33 @@ let bind_steel_steelf_req_unnormal (#a:Type)
   (#pre_f:pre_t) (#post_f:post_t a)
   (req_f:req_t pre_f) (ens_f:ens_t pre_f a post_f)
   (#pre_g:a -> pre_t)
+  (#pr:a -> prop)
   (req_g:(x:a -> req_t (pre_g x)))
   (frame_f:vprop)
-  (_:squash (can_be_split_forall (fun x -> post_f x `star` frame_f) pre_g))
+  (_:squash (can_be_split_forall_dep pr (fun x -> post_f x `star` frame_f) pre_g))
   (m0:rmem (pre_f `star` frame_f))
 = req_f (focus_rmem m0 pre_f) /\
   (forall (x:a) (m1:rmem (post_f x `star` frame_f)).
     (ens_f (focus_rmem m0 pre_f) x (focus_rmem m1 (post_f x)) /\ frame_equalities frame_f (focus_rmem m0 frame_f) (focus_rmem m1 frame_f)) ==>
-      (req_g x) (focus_rmem m1 (pre_g x)))
+      pr x /\ (req_g x) (focus_rmem m1 (pre_g x)))
 
 unfold
 let bind_steel_steelf_ens_unnormal (#a:Type) (#b:Type)
   (#pre_f:pre_t) (#post_f:post_t a)
   (req_f:req_t pre_f) (ens_f:ens_t pre_f a post_f)
   (#pre_g:a -> pre_t) (#post_g:a -> post_t b)
+  (#pr:a -> prop)
   (ens_g:(x:a -> ens_t (pre_g x) b (post_g x)))
   (frame_f:vprop)
   (post:post_t b)
-  (_:squash (can_be_split_forall (fun x -> post_f x `star` frame_f) pre_g))
+  (_:squash (can_be_split_forall_dep pr (fun x -> post_f x `star` frame_f) pre_g))
   (_: squash (can_be_split_post post_g post))
   (m0:rmem (pre_f `star` frame_f))
   (y:b)
   (m2:rmem (post y))
 = req_f (focus_rmem m0 pre_f) /\
   (exists (x:a) (m1:rmem (post_f x `star` frame_f)). (
+    pr x /\
     frame_equalities frame_f (focus_rmem m0 frame_f) (focus_rmem m1 frame_f)) /\
     ens_f (focus_rmem m0 pre_f) x (focus_rmem m1 (post_f x)) /\ (ens_g x) (focus_rmem m1 (pre_g x)) y (focus_rmem m2 (post_g x y)))
 
@@ -502,7 +515,8 @@ val bind_steel_steelf_aux (a:Type) (b:Type)
   (#req_g:(x:a -> req_t (pre_g x))) (#ens_g:(x:a -> ens_t (pre_g x) b (post_g x)))
   (#frame_f:vprop)
   (#post:post_t b)
-  (#p:squash (can_be_split_forall (fun x -> post_f x `star` frame_f) pre_g))
+  (#pr:a -> prop)
+  (#p:squash (can_be_split_forall_dep pr (fun x -> post_f x `star` frame_f) pre_g))
   (#p2: squash (can_be_split_post post_g post))
   (f:repr a pre_f post_f req_f ens_f)
   (g:(x:a -> repr b (pre_g x) (post_g x) (req_g x) (ens_g x)))
@@ -546,30 +560,35 @@ let bind_steelf_steel_req_unnormal (#a:Type)
   (#pre_f:pre_t) (#post_f:post_t a)
   (req_f:req_t pre_f) (ens_f:ens_t pre_f a post_f)
   (#pre_g:a -> pre_t)
+  (#pr:a -> prop)
   (req_g:(x:a -> req_t (pre_g x)))
   (frame_g:a -> vprop)
-  (_:squash (can_be_split_forall post_f (fun x -> pre_g x `star` frame_g x)))
+  (_:squash (can_be_split_forall_dep pr post_f (fun x -> pre_g x `star` frame_g x)))
   (m0:rmem pre_f)
 = req_f m0 /\
-  (forall (x:a) (m1:rmem (post_f x)). (
-    can_be_split_trans (post_f x) (pre_g x `star` frame_g x) (pre_g x);
-    ens_f m0 x m1 ==> (req_g x) (focus_rmem m1 (pre_g x))))
+  (forall (x:a) (m1:rmem (post_f x)).
+    ens_f m0 x m1 ==>
+      pr x /\
+      (can_be_split_trans (post_f x) (pre_g x `star` frame_g x) (pre_g x);
+      (req_g x) (focus_rmem m1 (pre_g x))))
 
 unfold
 let bind_steelf_steel_ens_unnormal (#a:Type) (#b:Type)
   (#pre_f:pre_t) (#post_f:post_t a)
   (req_f:req_t pre_f) (ens_f:ens_t pre_f a post_f)
   (#pre_g:a -> pre_t) (#post_g:a -> post_t b)
+  (#pr:a -> prop)
   (ens_g:(x:a -> ens_t (pre_g x) b (post_g x)))
   (frame_g:a -> vprop)
   (post:post_t b)
-  (_:squash (can_be_split_forall post_f (fun x -> pre_g x `star` frame_g x)))
+  (_:squash (can_be_split_forall_dep pr post_f (fun x -> pre_g x `star` frame_g x)))
   (_:squash (can_be_split_post (fun x y -> post_g x y `star` frame_g x) post))
   (m0:rmem pre_f)
   (y:b)
   (m2:rmem (post y))
 = req_f m0 /\
-  (exists (x:a) (m1:rmem (post_f x)). (
+  (exists (x:a) (m1:rmem (post_f x)).
+    pr x /\ (
     can_be_split_trans (post_f x) (pre_g x `star` frame_g x) (pre_g x);
     can_be_split_trans (post_f x) (pre_g x `star` frame_g x) (frame_g x);
     can_be_split_trans (post y) (post_g x y `star` frame_g x) (post_g x y);
@@ -584,7 +603,8 @@ val bind_steelf_steel_aux (a:Type) (b:Type)
   (#req_g:(x:a -> req_t (pre_g x))) (#ens_g:(x:a -> ens_t (pre_g x) b (post_g x)))
   (#frame_g:a -> vprop)
   (#post:post_t b)
-  (#p:squash (can_be_split_forall post_f (fun x -> pre_g x `star` frame_g x)))
+  (#pr:a -> prop)
+  (#p:squash (can_be_split_forall_dep pr post_f (fun x -> pre_g x `star` frame_g x)))
   (#p2:squash (can_be_split_post (fun x y -> post_g x y `star` frame_g x) post))
   (f:repr a pre_f post_f req_f ens_f)
   (g:(x:a -> repr b (pre_g x) (post_g x) (req_g x) (ens_g x)))
